theories/Decidability/UntypedSoundness.v
@@ -1,0 +1,81 @@
+(** * LogRel.Decidability.Soundness: the implementations imply the inductive predicates. *)
+From Coq Require Import Nat Lia Arith.
+From Equations Require Import Equations.
+From LogRel.AutoSubst Require Import core unscoped Ast Extra.
+From LogRel Require Import Utils BasicAst Context Notations UntypedReduction GenericTyping NormalForms.
+From LogRel Require Import AlgorithmicTyping UntypedAlgorithmicConversion.
+From LogRel.Decidability Require Import Functions UntypedFunctions Soundness.
+From PartialFun Require Import Monad PartialFun MonadExn.
+
+Import AlgorithmicTypingData.
+
+Set Universe Polymorphism.
+
+Section ConversionSound.
+
+  #[universes(polymorphic)]Definition uconv_sound_type
+    (x : uconv_state × term × term)
+    (r : exn errors unit) : Type :=
+  match x, r with
+  | _, (exception _) => True
+  | (tm_state,t,u), (success _) =>  [t ≅ u]
+  | (tm_red_state,t,u), (success _) =>
+      whnf t -> whnf u -> [t ≅h u]
+  | (ne_state,m,n), (success _) => [m ~ n]
+  end.
+
+  Lemma _implem_uconv_sound :
+    funrect _uconv (fun _ => True) uconv_sound_type.
+  Proof.
+    intros x _.
+    funelim (_uconv _); 
+      [ funelim (uconv_tm _) | funelim (uconv_tm_red _) | funelim (uconv_ne _) ].
+    all: intros ; cbn ; try easy ; cbn.
+    all: repeat (
+      match goal with
+      | |- True * _ => split ; [easy|..]
+      | |- forall x : exn _ _, _ => intros [|] ; [..|easy] ; cbn
+      | |- _ -> _ => cbn ; intros ?
+      | |- context [match ?t with | _ => _ end] => destruct t ; cbn ; try easy
+      | s : sort |- _ => destruct s
+      | H : graph wh_red _ _ |- _ => eapply red_sound in H as []
+      | H : (_,_,_) = (_,_,_) |- _ => injection H; clear H; intros; subst 
+      end).
+    all: try solve [now econstructor].
+    1-4: econstructor ; tea.
+    1-4: match goal with | H : whnf ?t |- whne ?t =>
+      now destruct H ; simp build_nf_view3 build_ty_view1 in Heq ; try solve [inversion Heq]
+      end.
+    eapply Nat.eqb_eq in Heq as ->.
+    now constructor.
+  Qed.
+
+  Corollary implem_conv_graph x r :
+    graph _uconv x r ->
+    uconv_sound_type x r.
+  Proof.
+    eapply funrect_graph.
+    1: now apply _implem_uconv_sound.
+    easy.
+  Qed.
+
+  Corollary implem_uconv_sound Γ T V :
+    graph uconv (Γ,T,V) ok ->
+    [T ≅ V].
+  Proof.
+    assert (funrect uconv (fun _ => True)
+      (fun '(Γ,T,V) r => match r with | success _ => [T ≅ V] | _ => True end)) as Hrect.
+    {
+     intros ? _.
+     funelim (uconv _) ; cbn.
+     intros [] ; cbn ; [|easy].
+     eintros ?%funrect_graph.
+     2: now apply _implem_uconv_sound.
+     all: now cbn in *.
+    }
+    eintros ?%funrect_graph.
+    2: eassumption.
+    all: now cbn in *.
+  Qed.
+
+End ConversionSound.
